proof/invariant-abstract/Deterministic_AI.thy
@@ -4144,8 +4144,6 @@ lemma set_mcpriority_valid_list[wp]:
 
 crunch (empty_fail)empty_fail[wp]: set_priority,set_mcpriority
 
-crunch valid_list[wp]: unbind_reply_in_ts,no_reply_in_ts valid_list
-
 lemma reply_push_valid_list[wp]:
   "\<lbrace>valid_list\<rbrace> reply_push caller callee reply_ptr can_donate \<lbrace>\<lambda>_. valid_list\<rbrace>"
   by (wpsimp simp: reply_push_def
